# 信号与系统

- [信号与系统](#信号与系统)
  - [第十章](#第十章)
    - [10.1 (a) (b)](#101-a-b)
    - [10.3](#103)
    - [10.6](#106)
    - [10.11](#1011)
    - [10.14](#1014)
    - [10.20](#1020)
    - [10.33](#1033)
    - [10.42](#1042)


## 第十章

### 10.1 (a) (b)

![10.1](./10.1.png)

(a)

$$
|z| > \frac{1}{2}
$$

(b)

$$
|z| < \frac{1}{2}
$$

### 10.3

![10.3](./10.3.png)

$$
n_0 为任意实数 \\

|\alpha| = 2
$$

### 10.6

![10.6](./10.6.png)

(a) 不是

(b) 不是

(c) 不是

(d) 是

### 10.11

![10.11](./10.11.png)

$$
x[n] = 
\begin{cases}
  (\frac{1}{2})^n, & 0 \le n \le 9 \\
  0, & 其他
\end{cases}
$$

### 10.14

![10.14](./10.14.png)

(a)

$$
n_0 = 2
$$

(b)

$$
G(z) = (\frac{1 - z^{-6}}{z - 1})^2
$$

### 10.20

![10.20](./10.20.png)

(a)

$$
-(- \frac{1}{2})^n \ u[n]
$$

(b)

$$
\frac{1}{3}\{(-\frac{1}{2})^n \ u[n] + (\frac{1}{2})^{2n + 1} \ u[n]\}
$$

(c)

$$
\frac{1}{3} \{-(\frac{1}{2})^{n-1} \ u[n] + (\frac{1}{2})^{2n+1} \ u[n]\}
$$

### 10.33

![10.33](./10.33.png)

(a)

$$
H(z) = \frac{1}{1 - \frac{1}{2} z^{-1} + \frac{1}{4} z^{-2}}
$$

(b)

$$
X(z) = \frac{1}{1 - \frac{1}{2} z^{-1}}, |z| > \frac{1}{2}
\\
\begin{aligned}
  Y(z) & = H(z) \cdot X(z) \\
       & = \frac{1}{1 - \frac{1}{2} z^{-1}} \cdot \frac{1}{1 - \frac{1}{2} z^{-1} + \frac{1}{4} z^{-2}} \\
       & = \frac{1}{1 - \frac{1}{2} z^{-1}} + \frac{\frac{1}{2}z - 1}{1 - \frac{1}{2}z^{-1} + \frac{1}{4}z^{-2}} \\
\end{aligned}
\\
y[n] = (\frac{1}{2})^n \ {\rm u}[n] + \frac{2}{\sqrt{3}} \cdot (\frac{1}{2})^n \sin(\frac{\pi n}{3}) \ {\rm u}[n]
$$

### 10.42

![10.42](./10.42.png)

(a)

$$
\begin{aligned}
  & y(z) + 3z^{-1} \ y(z) = X(z) \Rightarrow y(z) = -\frac{3}{1 + 3z^{-1}} ,\ X(z) = 0 \\
  & 零输入响应：y_{0z}[n] = (-3)^{n + 1} \ {\rm u}[n] \\
  \\
  & X(z) = \frac{1}{1 - \frac{1}{2}z^{-1}} \\
  & y(z) + 3z^{-1} \ y(z) = \frac{1}{1 - \frac{1}{2}z^{-1}} \\
  & \begin{aligned}
      y[z] & = \frac{1}{1 - \frac{1}{2}z^{-1}} \cdot \frac{1}{1 + 3z^{-1}} \\
           & = \frac{1}{7} \cdot \frac{1}{1 - \frac{1}{2}z^{-1}} + \frac{6}{7} \cdot \frac{1}{1 + 3z^{-1}}
    \end{aligned} \\
  & y_{0z}[n] = \frac{1}{7} \cdot (\frac{1}{2})^{n} \ {\rm u}[n] + \frac{6}{7} \cdot (-3)^{n} \ {\rm u}[n]
\end{aligned}
$$

(b)

$$
y(z) - \frac{1}{2}z^{-1} \ y(z) - \frac{1}{2} y[-1] = x(z) - \frac{1}{2}z^{-1} \ x(z) \\
\Downarrow \\
y_{oz}[z] = 0, \quad y_{oz}[n] = 0 \\
\begin{aligned}
  & x(z) = \frac{1}{1 - z^{-1}} \\
  & y(z) - \frac{1}{2} \ y(z) = \frac{1}{1 - z^{-1}} - \frac{1}{2} \cdot \frac{z^{-1}}{1 - z^{-1}} \\
  & y(z) = \frac{1}{1 - z^{-1}} \\
  & y_{0z} = {\rm u}[n]
\end{aligned}
$$

(c)

$$
y(z) = \frac{1}{2}z^{-1} \ y(z) - \frac{1}{2}y[-1] = x(z) - \frac{1}{2}z^{-1} \ x(z) \\
\Downarrow \\
y_{0z}(z) = \frac{1}{2} \cdot \frac{1}{1 - \frac{1}{2}z^[-1]}, \quad y_{0z}[n] = (\frac{1}{2})^{n + 1} \ {\rm u}[n] \\
同上，得到 y_{0z}[n] = {\rm u} [n]
$$
